code cleanup, add comments

execution/tests/EscrowTests/EscrowTests.v
@@ -1,3 +1,8 @@
+(* QuickChick tests of the Escrow contract. The properties tested are:
+   - functional correctness (also proved in Escrow.v)
+   - the next_step field satisfies a certain ordering (e.g. buyer_commit -> buyer_confirm -> withdrawals)
+*)
+
 From ConCert Require Import Blockchain LocalBlockchain Escrow EscrowExtras.
 From ConCert Require Import Serializable.
 From ConCert Require Import ResultMonad.
@@ -17,30 +22,29 @@ Import ListNotations.
 Import RecordSetNotations.
 Close Scope string_scope. 
 
-(* First we derive decidable equality on NextStep *)
-Scheme Equality for NextStep.
-Instance nextstep_dec_eq : Dec_Eq NextStep.
-Proof. constructor. apply NextStep_eq_dec. Defined.
+Section TestSetup.
+  (* Fix seller and buyer *)
+  Definition seller := creator.
+  Definition buyer := person_1.
 
-(* Fix seller and buyer *)
-Definition seller := creator.
-Definition buyer := person_1.
+  Definition escrow_setup := {|
+    setup_buyer := buyer
+  |}.
 
-Definition escrow_setup := {|
-  setup_buyer := buyer
-|}.
-
-Definition deploy_escrow amount := create_deployment amount Escrow.contract escrow_setup.
-Definition escrow_contract_addr : Address := BoundedN.of_Z_const AddrSize 128%Z.
-Definition escrow_chain : ChainBuilder :=
-  unpack_result (TraceGens.add_block (lcb_initial AddrSize)
-  [
-    build_act creator (act_transfer buyer 10);
-    build_act seller (deploy_escrow 2)
-  ]).
+  Definition deploy_escrow amount := create_deployment amount Escrow.contract escrow_setup.
+  Definition escrow_contract_addr : Address := BoundedN.of_Z_const AddrSize 128%Z.
+  (* The initial blockchain with the escrow contract deployed, and with buyer balance = 10 *)
+  Definition escrow_chain : ChainBuilder :=
+    unpack_result (TraceGens.add_block (lcb_initial AddrSize)
+    [
+      build_act creator (act_transfer buyer 10);
+      build_act seller (deploy_escrow 2)
+    ]).
+    
+End TestSetup.
 
 (* To instantiate the EscrowGen module functor, we need to supply
-   an EscrowGensInfo module. *)
+    an EscrowGensInfo module. *)
 Module TestInfo <: EscrowGensInfo.
   Definition contract_addr := escrow_contract_addr.
   Definition gAccount := elems_ person_1 test_chain_addrs.
@@ -49,144 +53,209 @@ Module TestInfo <: EscrowGensInfo.
     elems_opt addrs.
 End TestInfo.
 Module MG := EscrowGens.EscrowGens TestInfo. Import MG.
+Section TestGenInstances.
+  
+  Definition forAllEscrowChainBuilder gEscrowTrace length cb := 
+    forAllChainBuilder length cb gEscrowTrace .
+  
+  (* For automation *)
+  Global Instance gEscrowChainBuilder : GenSized ChainBuilder := 
+  {|
+    arbitrarySized := gEscrowTraceBetter escrow_chain
+  |}.
+  Global Instance shrinkChainBuilder : Shrink ChainBuilder := {| shrink a := [a] |}.
 
-Definition forAllEscrowChainBuilder gEscrowTrace length cb := 
-  forAllChainBuilder length cb gEscrowTrace .
+End TestGenInstances.
 
-(* For automation *)
-Instance gEscrowChainBuilder : GenSized ChainBuilder := 
-{|
-  arbitrarySized := gEscrowTraceBetter escrow_chain
-|}.
-Instance shrinkChainBuilder : Shrink ChainBuilder := {| shrink a := [a] |}.
+Section TestProperties.
 
-(* Sample (gEscrowMsg escrow_chain). *)
-(* Sample (gEscrowTraceBetter escrow_chain 10). *)
-(* QuickChick (forAll (gEscrowTraceBetter escrow_chain 10) (fun cb =>
-  1 <? (chain_height cb)
-)). *)
-(* +++ Passed 10000 tests (0 discards) *)
+  (* This is the proposition we wish to test, but QuickChick cannot test arbitrary Props since they are not
+    decidable in general. Therefore, we define a boolean version, escrow_correct_bool, below and
+    show that it implies escrow_correct_Prop. We then test on escrow_correct_bool instead.
+    An alternative approach is to prove that escrow_correct_Prop is decidable, since QuickChick can test any
+    decidable proposition (by coercing it to a bool) *)
+  Local Open Scope Z_scope.
+  Definition escrow_correct_Prop {from to}
+                              (caddr : Address)
+                              (cstate : Escrow.State)
+                              (trace : ChainTrace from to) 
+                              (depinfo : DeploymentInfo Setup)
+                              (inc_calls : list (ContractCallInfo Msg)) : Prop := 
+    let item_worth := deployment_amount depinfo / 2 in
+    let seller := deployment_from depinfo in
+    let buyer := setup_buyer (deployment_setup depinfo) in
+    is_escrow_finished cstate = true ->
+    (buyer_confirmed inc_calls buyer = true /\
+      net_balance_effect trace caddr seller = item_worth /\
+      net_balance_effect trace caddr buyer = -item_worth \/
 
-(* This is the proposition we wish to test, but QuickChick cannot test arbitrary Props since they are not
-   decidable in general. Therefore, we define a boolean version, escrow_correct_bool, below and
-   show that it implies escrow_correct_Prop. We then test on escrow_correct_bool instead.
-   An alternative approach is to prove that escrow_correct_Prop is decidable, since QuickChick can test any
-   decidable proposition (by coercing it to a bool) *)
-Local Open Scope Z_scope.
-Definition escrow_correct_Prop {from to}
-                            (caddr : Address)
-                            (cstate : Escrow.State)
-                            (trace : ChainTrace from to) 
-                            (depinfo : DeploymentInfo Setup)
-                            (inc_calls : list (ContractCallInfo Msg)) : Prop := 
-  let item_worth := deployment_amount depinfo / 2 in
-  let seller := deployment_from depinfo in
-  let buyer := setup_buyer (deployment_setup depinfo) in
-  is_escrow_finished cstate = true ->
-  (buyer_confirmed inc_calls buyer = true /\
-    net_balance_effect trace caddr seller = item_worth /\
-    net_balance_effect trace caddr buyer = -item_worth \/
+      buyer_confirmed inc_calls buyer = false /\
+      net_balance_effect trace caddr seller = 0 /\
+      net_balance_effect trace caddr buyer = 0).
 
-    buyer_confirmed inc_calls buyer = false /\
-    net_balance_effect trace caddr seller = 0 /\
-    net_balance_effect trace caddr buyer = 0).
+  (* bool version of escrow_correct_Prop *)
+  Definition escrow_correct_bool {from to}
+                              (caddr : Address)
+                              (cstate : Escrow.State)
+                              (trace : ChainTrace from to) 
+                              (depinfo : DeploymentInfo Setup)
+                              (inc_calls : list (ContractCallInfo Msg)) := 
+    let item_worth := deployment_amount depinfo / 2 in
+    let seller := deployment_from depinfo in
+    let buyer := setup_buyer (deployment_setup depinfo) in
+    if is_escrow_finished cstate
+    then (buyer_confirmed inc_calls buyer &&
+      ((net_balance_effect trace caddr seller =? item_worth) &&
+      (net_balance_effect trace caddr buyer =? -item_worth)) 
+      ||
+      (negb (buyer_confirmed inc_calls buyer)) && 
+      ((net_balance_effect trace caddr seller =? 0) &&
+      (net_balance_effect trace caddr buyer =? 0)))
+    else true.
 
-(* bool version of escrow_correct_Prop *)
-Definition escrow_correct_bool {from to}
-                            (caddr : Address)
-                            (cstate : Escrow.State)
-                            (trace : ChainTrace from to) 
-                            (depinfo : DeploymentInfo Setup)
-                            (inc_calls : list (ContractCallInfo Msg)) := 
-  let item_worth := deployment_amount depinfo / 2 in
-  let seller := deployment_from depinfo in
-  let buyer := setup_buyer (deployment_setup depinfo) in
-  if is_escrow_finished cstate
-  then (buyer_confirmed inc_calls buyer &&
-    ((net_balance_effect trace caddr seller =? item_worth) &&
-    (net_balance_effect trace caddr buyer =? -item_worth)) 
-    ||
-    (negb (buyer_confirmed inc_calls buyer)) && 
-    ((net_balance_effect trace caddr seller =? 0) &&
-    (net_balance_effect trace caddr buyer =? 0)))
-  else true.
+  (* We show that the bool version implies the propositional version
+    of the correctness property. *)
+  Lemma escrow_correct_bool_refl_prop {from to}
+                                      (caddr : Address)
+                                      (cstate : Escrow.State)
+                                      (trace : ChainTrace from to) 
+                                      (depinfo : DeploymentInfo Setup)
+                                      (inc_calls : list (ContractCallInfo Msg)) : 
+    escrow_correct_bool caddr cstate trace depinfo inc_calls = true <->
+    escrow_correct_Prop caddr cstate trace depinfo inc_calls.
+  Proof. 
+    unfold escrow_correct_bool.
+    split.
+    - destruct (is_escrow_finished cstate) eqn:H1.
+      + unfold escrow_correct_Prop. 
+        intros. 
+        propify. 
+        apply H.
+      + intros. unfold escrow_correct_Prop. 
+        left. rewrite H1 in H0.
+        inversion H0.
+    - destruct (is_escrow_finished cstate) eqn:H1.
+      + unfold escrow_correct_Prop. 
+        propify. 
+        intros. 
+        repeat rewrite Z.eqb_eq.
+        apply H.
+        apply H1.
+      + intros. reflexivity.
+  Qed.
 
-(* We show that the bool version implies the propositional version
-   of the correctness property. *)
-Lemma escrow_correct_bool_impl_prop {from to}
-                                    (caddr : Address)
-                                    (cstate : Escrow.State)
-                                    (trace : ChainTrace from to) 
-                                    (depinfo : DeploymentInfo Setup)
-                                    (inc_calls : list (ContractCallInfo Msg)) : 
-  escrow_correct_bool caddr cstate trace depinfo inc_calls = true ->
-  escrow_correct_Prop caddr cstate trace depinfo inc_calls.
-Proof. 
-  unfold escrow_correct_bool.
-  destruct (is_escrow_finished cstate) eqn:H1.
-  - unfold escrow_correct_Prop. 
-    intros. 
-    propify. 
-    apply H.
-  - intros. unfold escrow_correct_Prop. left. rewrite H1 in H0. inversion H0. 
-Qed.
+  (* Finally, we can show that escrow_correct_Prop is decidable (using escrow_correct_bool as 
+    the decision procedure).  *)
+  Global Instance escrow_correct_P_dec {from to caddr cstate trace depinfo inc_calls} 
+    : Dec (@escrow_correct_Prop from to caddr cstate trace depinfo inc_calls).
+  Proof. 
+    constructor. unfold ssrbool.decidable.
+    destruct (escrow_correct_bool caddr cstate trace depinfo inc_calls) eqn:H.
+    - left. apply escrow_correct_bool_refl_prop. apply H.
+    - right. 
+      unfold not. 
+      intros.
+      apply escrow_correct_bool_refl_prop in H0.
+      eauto.
+  Defined.
 
-Lemma escrow_correct_bool_false_impl_prop {from to}
-(caddr : Address)
-(cstate : Escrow.State)
-(trace : ChainTrace from to) 
-(depinfo : DeploymentInfo Setup)
-(inc_calls : list (ContractCallInfo Msg)) : 
-  escrow_correct_bool caddr cstate trace depinfo inc_calls = false ->
-  ~(escrow_correct_Prop caddr cstate trace depinfo inc_calls).
-Proof. 
-  unfold escrow_correct_bool.
-  destruct (is_escrow_finished cstate) eqn:H1.
-  - unfold escrow_correct_Prop. 
-    propify. 
-    intros.
-    repeat rewrite Z.eqb_neq in H.
-    intuition.
-  - intros. unfold escrow_correct_Prop. eauto. 
-Qed.
+  Global Instance escrow_correct_P_checkable {from to caddr cstate trace depinfo inc_calls}
+    : Checkable (@escrow_correct_Prop from to caddr cstate trace depinfo inc_calls).
+  Proof. apply testDec. Defined.
 
-(* Finally, we can show that escrow_correct_Prop is decidable (using escrow_correct_bool as 
-   the decision procedure).  *)
-Instance escrow_correct_P_dec {from to caddr cstate trace depinfo inc_calls} 
-  : Dec (@escrow_correct_Prop from to caddr cstate trace depinfo inc_calls).
-Proof. 
-  constructor. unfold ssrbool.decidable. 
-  destruct (escrow_correct_bool caddr cstate trace depinfo inc_calls) eqn:H.
-  - left. apply escrow_correct_bool_impl_prop. apply H.
-  - right. 
-    unfold not. 
-    intros.
-    apply escrow_correct_bool_false_impl_prop in H.
-    contradiction.
-Defined.
+  Notation "a ===> f" := (isSomeCheck a f) (at level 44).
 
-Instance escrow_correct_P_checkable {from to caddr cstate trace depinfo inc_calls}
-  : Checkable (@escrow_correct_Prop from to caddr cstate trace depinfo inc_calls).
-Proof. apply testDec. Defined.
-
-(* Wrapper for escrow_correct_bool. This is the Checker we will run QC on. *)
-Definition escrow_correct_P (cb : ChainBuilder) := 
-  let trace := builder_trace cb in
-  let depinfo' := deployment_info Escrow.Setup trace escrow_contract_addr in
-  let inc_calls' := incoming_calls Escrow.Msg trace escrow_contract_addr in
-  isSomeCheck depinfo' (fun depinfo =>
-    isSomeCheck inc_calls' (fun inc_calls =>
+  (* Wrapper for escrow_correct_bool. This is the Checker we will run QC on. *)
+  Definition escrow_correct_P (cb : ChainBuilder) := 
+    let trace := builder_trace cb in
+    let depinfo' := deployment_info Escrow.Setup trace escrow_contract_addr in
+    let inc_calls' := incoming_calls Escrow.Msg trace escrow_contract_addr in
+    depinfo'  ===>  (fun depinfo =>
+    inc_calls' ===>  (fun inc_calls =>
       match get_contract_state Escrow.State cb escrow_contract_addr with
-      | Some cstate => is_escrow_finished cstate ==>
+      (* main part of the property: *)
+      | Some cstate => 
+        is_escrow_finished cstate ==>
         ((escrow_correct_Prop escrow_contract_addr cstate trace depinfo inc_calls)?)
       | None => checker false
       end
-    )
-  ).
+    )).
 
-Extract Constant defNumDiscards => "(3 * defNumTests)".
+  (* we derive decidable equality on NextStep *)
+  Scheme Equality for NextStep.
+  Instance nextstep_dec_eq : Dec_Eq NextStep.
+  Proof. constructor. apply NextStep_eq_dec. Defined.
+  
+  Definition escrow_next_states {from to} 
+                                (escrow_caddr : Address) 
+                                (trace : ChainTrace from to) : list NextStep :=
+    let fix rec {from to} (trace : ChainTrace from to) acc :=
+      match trace with
+      | snoc trace' step => 
+        match acc, get_contract_state Escrow.State to escrow_caddr with
+        | nextstep::_, Some state => if (nextstep = state.(next_step))?
+                                     then rec trace' acc
+                                     else rec trace' (state.(next_step) :: acc)
+        | [], Some state => rec trace' (state.(next_step) :: acc)
+        | _, _ => rec trace' acc
+        end 
+      | clnil => acc
+      end in 
+  rec trace [].
 
-QuickChick (forAllEscrowChainBuilder gEscrowTrace 7 escrow_chain escrow_correct_P).
+  (* We want to see what the length of the generated sequences of next_step are,
+  so we use QuickChick's 'collect' to collect length distribution statistics *)
+  Definition collect_steps_length_distribution g :=
+  forAll (g escrow_chain 10%nat) (fun cb =>
+  collect (length (escrow_next_states escrow_contract_addr (cb.(builder_trace))))
+  true).
+  (* QuickChick (collect_steps_length_distribution gEscrowTrace). *)
+  (* 
+  4812 : 2
+  2470 : 1
+  2244 : 3
+  474 : 4
+  +++ Passed 10000 tests (0 discards) *)
+  (* QuickChick (collect_steps_length_distribution gEscrowTraceBetter). *)
+  (* 
+  6636 : 4
+  3364 : 2
+  +++ Passed 10000 tests (0 discards) *)
+
+  (* We see that the "better" generator more often generates the full sequence of states, namely the sequence:
+  buyer_commit -> buyer_confirm -> withdrawals -> no_next_step
+  The sequence of length 2 is the sequence:
+  buyer_commit -> no_next_step
+  Corresponding to the case where the seller withdraws their funds before the buyer commits & confirms their purchase. *)
+
+  Fixpoint is_valid_step_sequence_fix steps prev_step :=
+  match prev_step, steps with
+  | _, [] => true
+  | None, step::steps' => is_valid_step_sequence_fix steps' (Some step) 
+  | Some prev_step, step::steps' => match prev_step, step with
+          | buyer_commit, buyer_confirm
+          | buyer_commit, no_next_step 
+          | buyer_confirm, withdrawals
+          | withdrawals, no_next_step => is_valid_step_sequence_fix steps' (Some step)
+          | _, _ => false
+          end
+  end.
+
+  Definition is_valid_step_sequence steps := 
+  is_valid_step_sequence_fix steps None.
+
+  (* Test property *)
+  Conjecture escrow_valid_steps_P : forall trace : {to : ChainState & ChainTrace empty_state to},
+  let steps := escrow_next_states escrow_contract_addr (projT2 trace) in
+  is_valid_step_sequence steps = true.
+
+End TestProperties.
+
+(* ---------- Test execution ---------- *)
+
+Extract Constant defNumDiscards => "(2 * defNumTests)".
+
+(* QuickChick (forAllEscrowChainBuilder gEscrowTrace 7 escrow_chain escrow_correct_P). *)
 (* *** Gave up! Passed only 8598 tests
 Discarded: 20000 *)
 
@@ -198,190 +267,6 @@ Discarded: 20000 *)
 (* +++ Passed 10000 tests (40 discards) *)
 (* Not sure where the 40 discards come from, but it's an acceptable amount for sure... *)
 
-Definition escrow_next_states {from to} 
-                              (escrow_caddr : Address) 
-                              (trace : ChainTrace from to) : list NextStep :=
-  let fix rec {from to} (trace : ChainTrace from to) acc :=
-    match trace with
-    | snoc trace' step => match acc, get_contract_state Escrow.State to escrow_caddr with
-                          | nextstep::_, Some state => 
-                            if (nextstep = state.(next_step))?
-                            then rec trace' acc
-                            else rec trace' (state.(next_step) :: acc)
-                          | [], Some state => rec trace' (state.(next_step) :: acc)
-                          | _, _ => rec trace' acc
-                          end 
-    | clnil => acc
-    end in rec trace [].
-
-(* We want to see what the length of the generated sequences of next_step are,
-   so we use QuickChick's 'collect' to collect length distribution statistics *)
-Definition collect_steps_length_distribution g :=
-  forAll (g escrow_chain 10%nat) (fun cb =>
-    collect (length (escrow_next_states escrow_contract_addr (cb.(builder_trace))))
-    true).
-
-(* QuickChick (collect_steps_length_distribution gEscrowTrace). *)
-(* 
-4812 : 2
-2470 : 1
-2244 : 3
-474 : 4
-+++ Passed 10000 tests (0 discards) *)
-(* QuickChick (collect_steps_length_distribution gEscrowTraceBetter). *)
-(* 
-6636 : 4
-3364 : 2
-+++ Passed 10000 tests (0 discards) *)
-
-(* We see that the "better" generator more often generates the full sequence of states, namely the sequence:
-   buyer_commit -> buyer_confirm -> withdrawals -> no_next_step
-   The sequence of length 2 is the sequence:
-   buyer_commit -> no_next_step
-   Corresponding to the case where the seller withdraws their funds before the buyer commits & confirms their purchase. *)
-
-Fixpoint is_valid_step_sequence_fix steps prev_step :=
-  match prev_step, steps with
-  | _, [] => true
-  | None, step::steps' => is_valid_step_sequence_fix steps' (Some step) 
-  | Some prev_step, step::steps' => match prev_step, step with
-                                    | buyer_commit, buyer_confirm
-                                    | buyer_commit, no_next_step 
-                                    | buyer_confirm, withdrawals
-                                    | withdrawals, no_next_step => is_valid_step_sequence_fix steps' (Some step)
-                                    | _, _ => false
-                                    end
-  end.
-
-Definition is_valid_step_sequence steps := 
-  is_valid_step_sequence_fix steps None.
-
-
-Conjecture escrow_valid_steps_P : forall trace : {to : ChainState & ChainTrace empty_state to},
-  let steps := escrow_next_states escrow_contract_addr (projT2 trace) in
-  is_valid_step_sequence steps = true.
 (* Note that we are implicitly using the "better" generator here to generate arbitrary ChainTraces *)
 (* QuickChick escrow_valid_steps_P. *)
 (* +++ Passed 10000 tests (0 discards) *)
-
-Corollary escrow_correct
-            {ChainBuilder : ChainBuilderType}
-            prev new header acts :
-    builder_add_block prev header acts = Ok new ->
-    let trace := builder_trace new in
-    forall caddr,
-      env_contracts new caddr = Some (Escrow.contract : WeakContract) ->
-      let next_states := escrow_next_states caddr trace in
-      is_valid_step_sequence next_states = true.
-Proof.
-Admitted.  (* intros after_add trace caddr escrow_at_caddr next_states. *)
-  (* unfold trace.
-  contract_induction.
-  contract_induction; cbn in *; intros.
-  - (* New block *)
-    auto.
-  - (* Deployment *)
-    unfold Escrow.init in *.
-    destruct (address_eqb_spec (setup_buyer setup) (ctx_from ctx));
-      cbn in *; try congruence.
-    destruct (ctx_amount ctx =? 0) eqn:amount_some; cbn in *; try congruence.
-    destruct (Z.even (ctx_amount ctx)) eqn:amount_even; cbn in *; try congruence.
-    inversion init_some; subst; clear init_some.
-    cbn.
-    assert (2 * (ctx_amount ctx / 2) > 0 -> ctx_amount ctx / 2 > 0) by lia.
-    enough (2 * (ctx_amount ctx / 2) > 0 /\
-            ctx_amount ctx = 2 * (ctx_amount ctx / 2)) by tauto.
-    assert (ctx_amount ctx mod 2 = 0).
-    {
-      rewrite Zeven_mod in amount_even.
-      unfold Zeq_bool in *.
-      destruct_match eqn:amount_mod_2 in amount_even; try congruence; auto.
-      destruct (Z.compare_spec (ctx_amount ctx mod 2) 0); auto; try congruence.
-    }
-    rewrite <- (Z_div_exact_2 (ctx_amount ctx) 2) by (auto; lia).
-    split; auto.
-    instantiate (DeployFacts := fun _ ctx => ctx_amount ctx >= 0);
-      subst DeployFacts; cbn in *.
-    apply Z.eqb_neq in amount_some.
-    lia. *)
-
-(* 
-    intros after_add trace caddr escrow_at_caddr.
-    cbn in *.
-    pose proof (escrow_correct_strong _ caddr trace escrow_at_caddr) as general.
-    cbn in general.
-    destruct general as
-        [cstate [depinfo [inc_calls [? [? [? [? [? [? [? [? [_ IH]]]]]]]]]]]].
-    exists depinfo, cstate, inc_calls.
-    do 3 (split; [tauto|]).
-    intros is_finished.
-    unfold is_escrow_finished in *.
-    destruct (next_step cstate); try congruence; clear is_finished.
-    unfold net_balance_effect, money_to.
-    assert (inc_txs:
-              forall addr,
-                sumZ tx_amount (txs_from addr (incoming_txs trace caddr)) =
-                sumZ (fun '(a, b, c) => c)
-                     (filter (fun '(from, _, _) => (from =? addr)%address)
-                             (map (fun tx => (tx_from tx, tx_to tx, tx_amount tx))
-                                  (incoming_txs trace caddr)))).
-    {
-      intros addr.
-      induction (incoming_txs trace caddr) as [|hd tl IH'].
-      - reflexivity.
-      - rewrite txs_from_cons.
-        cbn.
-        destruct_address_eq; cbn in *; rewrite IH'; reflexivity.
-    }
-
-    repeat rewrite inc_txs; clear inc_txs.
-    rewrite (incoming_txs_contract caddr _ trace _ depinfo _ inc_calls) by assumption.
-    repeat rewrite filter_app, sumZ_app.
-    cbn.
-    rewrite address_eq_refl.
-    rewrite address_eq_ne by auto.
-    cbn.
-    rewrite 2!filter_map, 2!sumZ_map.
-
-    set (buyer_addr := setup_buyer (deployment_setup depinfo)) in *.
-    set (seller_addr := deployment_from depinfo) in *.
-
-    unfold money_to, transfer_acts_to in IH.
-    cbn in IH.
-
-    change (fun a => call_amount a) with (@call_amount _ Msg).
-
-    destruct IH as [IH | IH]; [left|right].
-    - split; [tauto|].
-      remember (build_call_info _ _ (Some commit_money)) as commitment.
-      assert (Hsum :
-                forall f,
-                  sumZ call_amount (filter f inc_calls) =
-                  sumZ call_amount (filter f [commitment])).
-      {
-        intros f.
-        destruct IH as [_ [<- ?]].
-        clear -inc_calls.
-        induction inc_calls as [|hd tl IH']; auto.
-        cbn.
-        destruct (Z.eqb_spec (call_amount hd) 0) as [zero_amount|].
-        - cbn.
-          destruct (f hd); cbn; try rewrite zero_amount; rewrite IH'; auto.
-        - cbn.
-          destruct (f hd); cbn; rewrite IH'; auto.
-      }
-
-      rewrite 2!Hsum; clear Hsum; subst commitment; cbn in *.
-      rewrite address_eq_refl, address_eq_ne by auto.
-      cbn.
-      destruct IH as [_ [_ [? ?]]].
-      split; lia.
-    - destruct IH as [-> IH].
-      cbn.
-      rewrite address_eq_refl, address_eq_ne by auto.
-      cbn.
-      split; [auto|].
-      split; lia.
-  Qed.
-
-*)
